wip: exp_four_fw

specs/Spec.Exponentiation.fsti
@@ -172,6 +172,11 @@ val exp_fw_lemma: #t:Type -> k:concrete_ops t -> a:t -> bBits:nat -> b:nat{b < p
   Lemma (k.to.refl (exp_fw k a bBits b l) == S.exp_fw k.to.comm_monoid (k.to.refl a) bBits b l)
 
 
+///  Multi-Exponentiation
+
+// Double exponentiation [a1^b1 `mul` a2^b2]
+//-------------------------------------------
+
 let exp_double_fw_acc0 (#t:Type) (k:concrete_ops t)
   (a1:t) (bBits:nat) (b1:nat{b1 < pow2 bBits})
   (a2:t) (b2:nat{b2 < pow2 bBits}) (l:pos{bBits % l <> 0}) : t
@@ -207,3 +212,62 @@ val exp_double_fw_lemma: #t:Type -> k:concrete_ops t
   -> a2:t -> b2:nat{b2 < pow2 bBits} -> l:pos ->
   Lemma (k.to.refl (exp_double_fw k a1 bBits b1 a2 b2 l) ==
     S.exp_double_fw k.to.comm_monoid (k.to.refl a1) bBits b1 (k.to.refl a2) b2 l)
+
+// [a1^b1 `mul` a2^b2 `mul` a3^b3 `mul` a4^b4]
+//----------------------------------------------
+
+let exp_four_fw_acc0 (#t:Type) (k:concrete_ops t)
+  (a1:t) (bBits:nat) (b1:nat{b1 < pow2 bBits})
+  (a2:t) (b2:nat{b2 < pow2 bBits})
+  (a3:t) (b3:nat{b3 < pow2 bBits})
+  (a4:t) (b4:nat{b4 < pow2 bBits})
+  (l:pos{bBits % l <> 0}) : t
+ =
+  let acc_a1 = exp_fw_acc0 k a1 bBits b1 l in
+  let acc_a2 = exp_fw_acc0 k a2 bBits b2 l in
+  let acc_a3 = exp_fw_acc0 k a3 bBits b3 l in
+  let acc_a4 = exp_fw_acc0 k a4 bBits b4 l in
+  let acc = k.mul acc_a1 acc_a2 in
+  let acc = k.mul acc acc_a3 in
+  let acc = k.mul acc acc_a4 in
+  acc
+
+
+let exp_four_fw_f (#t:Type) (k:concrete_ops t)
+  (a1:t) (bBits:nat) (b1:nat{b1 < pow2 bBits})
+  (a2:t) (b2:nat{b2 < pow2 bBits})
+  (a3:t) (b3:nat{b3 < pow2 bBits})
+  (a4:t) (b4:nat{b4 < pow2 bBits})
+  (l:pos) (i:nat{i < bBits / l}) (acc:t) : t
+ =
+  let acc = exp_fw_f k a1 bBits b1 l i acc in
+  let acc = mul_acc_pow_a_bits_l k a2 bBits b2 l i acc in
+  let acc = mul_acc_pow_a_bits_l k a3 bBits b3 l i acc in
+  let acc = mul_acc_pow_a_bits_l k a4 bBits b4 l i acc in
+  acc
+
+
+let exp_four_fw (#t:Type) (k:concrete_ops t)
+  (a1:t) (bBits:nat) (b1:nat{b1 < pow2 bBits})
+  (a2:t) (b2:nat{b2 < pow2 bBits})
+  (a3:t) (b3:nat{b3 < pow2 bBits})
+  (a4:t) (b4:nat{b4 < pow2 bBits})
+  (l:pos) : t
+ =
+  let acc0 =
+    if bBits % l = 0 then one ()
+    else exp_four_fw_acc0 k a1 bBits b1 a2 b2 a3 b3 a4 b4 l in
+
+  Loops.repeati (bBits / l)
+    (exp_four_fw_f k a1 bBits b1 a2 b2 a3 b3 a4 b4 l) acc0
+
+
+val exp_four_fw_lemma: #t:Type -> k:concrete_ops t
+  -> a1:t -> bBits:nat -> b1:nat{b1 < pow2 bBits}
+  -> a2:t -> b2:nat{b2 < pow2 bBits}
+  -> a3:t -> b3:nat{b3 < pow2 bBits}
+  -> a4:t -> b4:nat{b4 < pow2 bBits}
+  -> l:pos ->
+  Lemma (k.to.refl (exp_four_fw k a1 bBits b1 a2 b2 a3 b3 a4 b4 l) ==
+    S.exp_four_fw k.to.comm_monoid (k.to.refl a1) bBits b1 (k.to.refl a2)
+      b2 (k.to.refl a3) b3 (k.to.refl a4) b4 l)
